Splinter/BlockLayer/BlockCrashTolerantJournal.i.dfy
@@ -10,7 +10,7 @@ module BlockCrashTolerantJournal {
   import opened Options
   import opened ValueMessage
   import opened KeyType
-  import opened StampedMapMod
+  import opened StampedMod
   import opened MsgHistoryMod
   import opened LSNMod
   import opened GenericDisk
