Splinter/BlockLayer/BlockCrashTolerantMapRefinement.i.dfy
@@ -8,7 +8,7 @@ module BlockCrashTolerantMapRefinement {
   import opened Options
   import opened ValueMessage
   import opened KeyType
-  import opened StampedMapMod
+  import opened StampedMod
   import opened MsgHistoryMod
   import opened LSNMod
   import CrashTolerantMap 
